backend/Unusedglobproof.v
@@ -1439,16 +1439,15 @@ Proof.
   * unfold init_meminj.
   apply Genv.init_mem_stack in IM.
   unfold struct_meminj.
-  assert (~sup_In (Stack n f p0 p1) sup_empty) by (apply Mem.empty_in).
+  assert (~sup_In (Stack n f p0 p1) sup_init) by (apply Mem.empty_in).
   assert (~sup_In (Stack n f p0 p1) (Mem.support m)).
-  simpl. rewrite IM. destruct p0; destr. simpl. intros [H1 H2]. auto.
-  simpl. destruct n; auto.
-  simpl. repeat destr. destruct n0; simpl in Heqo; congruence.
+  simpl. rewrite IM. destr. destruct p0; simpl. intros [H1 H2]. auto.
+  destruct n0; simpl. congruence. congruence.
   simpl. repeat destr.
-  apply Genv.invert_find_symbol in Heqo. apply Genv.genv_vars_eq in Heqo. inv Heqo.
-  apply Genv.invert_find_symbol in Heqo. apply Genv.genv_vars_eq in Heqo. inv Heqo.
-  repeat destr_in Heqb.
-  repeat destr_in Heqb.
+  + destr_in Heqb0.
+  + apply Genv.invert_find_symbol in Heqo. apply Genv.genv_vars_eq in Heqo. inv Heqo.
+  + apply Genv.invert_find_symbol in Heqo. apply Genv.genv_vars_eq in Heqo. inv Heqo.
+  + destr_in Heqb.
   * unfold init_meminj. unfold struct_meminj. simpl.
     repeat destr.
     -
@@ -1547,9 +1546,10 @@ Proof.
   constructor. auto.
   erewrite <- Genv.init_mem_genv_sup by eauto. apply Mem.sup_include_refl.
   erewrite <- Genv.init_mem_genv_sup by eauto. apply Mem.sup_include_refl.
-  intros. destruct (eq_block b1 (Stack 0%nat None nil 1)). subst. rewrite SID in X. rewrite SID1 in X.
+  intros. destruct (eq_block b1 (Stack Mem.pid None nil 1)). subst. rewrite SID in X. rewrite SID1 in X.
   rewrite X in H5. inv H5.
-  simpl. rewrite STK1. rewrite STK2. rewrite SID. rewrite SID1. simpl. split. lia. lia. rewrite Y in H5. congruence. auto.
+  simpl. rewrite STK1. rewrite STK2. rewrite SID. rewrite SID1. simpl.
+  split. intro. inv H5. inv H8. intro. inv H5. inv H8. rewrite Y in H5. congruence. auto.
   congruence.
   unfold Mem.stackeq.
   split. congruence.
